<?xml version="1.0"?>
<rdf:RDF xmlns="http://www.semanticweb.org/lenovo/ontologies/2017/11/sensorSensingOntology/"
     xml:base="http://www.semanticweb.org/lenovo/ontologies/2017/11/sensorSensingOntology/"
     xmlns:ExtendedRelationOntology="http://www.ontologylibrary.mil/CommonCore/Upper/ExtendedRelationOntology#"
     xmlns:rdf="http://www.w3.org/1999/02/22-rdf-syntax-ns#"
     xmlns:owl="http://www.w3.org/2002/07/owl#"
     xmlns:oboInOwl="http://www.geneontology.org/formats/oboInOwl#"
     xmlns:xml="http://www.w3.org/XML/1998/namespace"
     xmlns:xsd="http://www.w3.org/2001/XMLSchema#"
     xmlns:rdfs="http://www.w3.org/2000/01/rdf-schema#"
     xmlns:obo="http://purl.obolibrary.org/obo/"
     xmlns:foaf="http://xmlns.com/foaf/0.1/"
     xmlns:dc="http://purl.org/dc/elements/1.1/">
    <owl:Ontology rdf:about="http://www.semanticweb.org/lenovo/ontologies/2017/11/sensorSensingOntology">
        <owl:imports rdf:resource="http://purl.obolibrary.org/obo/bfo/2.0/bfo.owl"/>
    </owl:Ontology>
    


    <!-- 
    ///////////////////////////////////////////////////////////////////////////////////////
    //
    // Object Properties
    //
    ///////////////////////////////////////////////////////////////////////////////////////
     -->

    


    <!-- http://www.obofoundry.org/ro/ro.owl#has_part -->

    <owl:ObjectProperty rdf:about="http://www.obofoundry.org/ro/ro.owl#has_part">
        <rdfs:subPropertyOf rdf:resource="http://www.w3.org/2002/07/owl#topObjectProperty"/>
    </owl:ObjectProperty>
    


    <!-- http://www.semanticweb.org/lenovo/ontologies/2017/10/memon_00001060 -->

    <owl:ObjectProperty rdf:about="http://www.semanticweb.org/lenovo/ontologies/2017/10/memon_00001060">
        <rdfs:label xml:lang="fr">on platform</rdfs:label>
    </owl:ObjectProperty>
    


    <!-- http://www.semanticweb.org/lenovo/ontologies/2017/10/memon_00001064 -->

    <owl:ObjectProperty rdf:about="http://www.semanticweb.org/lenovo/ontologies/2017/10/memon_00001064">
        <rdfs:label xml:lang="en">produced by</rdfs:label>
    </owl:ObjectProperty>
    


    <!-- http://www.semanticweb.org/lenovo/ontologies/2017/10/memon_00001073 -->

    <owl:ObjectProperty rdf:about="http://www.semanticweb.org/lenovo/ontologies/2017/10/memon_00001073">
        <rdfs:domain rdf:resource="http://www.semanticweb.org/lenovo/ontologies/2017/10/memon_00001003"/>
        <rdfs:label xml:lang="fr">observes</rdfs:label>
    </owl:ObjectProperty>
    


    <!-- 
    ///////////////////////////////////////////////////////////////////////////////////////
    //
    // Classes
    //
    ///////////////////////////////////////////////////////////////////////////////////////
     -->

    


    <!-- http://purl.obolibrary.org/obo/RO_0002577 -->

    <owl:Class rdf:about="http://purl.obolibrary.org/obo/RO_0002577">
        <rdfs:subClassOf rdf:resource="http://purl.obolibrary.org/obo/BFO_0000040"/>
        <obo:IAO_0000115 xml:lang="en">A material entity consisting of multiple components that are causally integrated.</obo:IAO_0000115>
        <obo:IAO_0000119>http://www.jbiomedsem.com/content/4/1/43</obo:IAO_0000119>
        <rdfs:label>system</rdfs:label>
    </owl:Class>
    


    <!-- http://www.ontologylibrary.mil/CommonCore/Mid/ArtifactOntology#AcousticSensor -->

    <owl:Class rdf:about="http://www.ontologylibrary.mil/CommonCore/Mid/ArtifactOntology#AcousticSensor">
        <rdfs:subClassOf rdf:resource="http://www.ontologylibrary.mil/CommonCore/Mid/ArtifactOntology#Sensor"/>
        <obo:IAO_0000115>A Sensor that is designed to measure sound levels.</obo:IAO_0000115>
        <rdfs:label xml:lang="en">acoustic sensor</rdfs:label>
    </owl:Class>
    


    <!-- http://www.ontologylibrary.mil/CommonCore/Mid/ArtifactOntology#Artifact -->

    <owl:Class rdf:about="http://www.ontologylibrary.mil/CommonCore/Mid/ArtifactOntology#Artifact">
        <rdfs:subClassOf rdf:resource="http://purl.obolibrary.org/obo/BFO_0000030"/>
        <obo:IAO_0000115>An Object that was designed by some Agent to realize a certain function.</obo:IAO_0000115>
        <rdfs:label>Artifact</rdfs:label>
    </owl:Class>
    


    <!-- http://www.ontologylibrary.mil/CommonCore/Mid/ArtifactOntology#Sensor -->

    <owl:Class rdf:about="http://www.ontologylibrary.mil/CommonCore/Mid/ArtifactOntology#Sensor">
        <rdfs:subClassOf rdf:resource="http://www.semanticweb.org/lenovo/ontologies/2017/10/memon_00001003"/>
        <obo:IAO_0000115>A Transducer that is designed to detect events or changes in its environment, and then provide a corresponding output.</obo:IAO_0000115>
    </owl:Class>
    


    <!-- http://www.ontologylibrary.mil/CommonCore/Mid/ArtifactOntology#SensorSystem -->

    <owl:Class rdf:about="http://www.ontologylibrary.mil/CommonCore/Mid/ArtifactOntology#SensorSystem">
        <rdfs:subClassOf rdf:resource="http://purl.obolibrary.org/obo/RO_0002577"/>
        <rdfs:subClassOf rdf:resource="http://www.semanticweb.org/lenovo/ontologies/2017/10/memon_00001003"/>
        <rdfs:subClassOf>
            <owl:Restriction>
                <owl:onProperty rdf:resource="http://www.obofoundry.org/ro/ro.owl#has_part"/>
                <owl:someValuesFrom rdf:resource="http://www.ontologylibrary.mil/CommonCore/Mid/ArtifactOntology#Sensor"/>
            </owl:Restriction>
        </rdfs:subClassOf>
        <rdfs:label>Sensor System</rdfs:label>
    </owl:Class>
    


    <!-- http://www.ontologylibrary.mil/CommonCore/Mid/ArtifactOntology#Transducer -->

    <owl:Class rdf:about="http://www.ontologylibrary.mil/CommonCore/Mid/ArtifactOntology#Transducer">
        <rdfs:subClassOf rdf:resource="http://www.ontologylibrary.mil/CommonCore/Mid/ArtifactOntology#Artifact"/>
        <obo:IAO_0000115>An Artifact that is designed to convert one form of energy to another.</obo:IAO_0000115>
    </owl:Class>
    


    <!-- http://www.ontologylibrary.mil/CommonCore/Mid/InformationEntityOntology#DescriptiveInformationContentEntity -->

    <owl:Class rdf:about="http://www.ontologylibrary.mil/CommonCore/Mid/InformationEntityOntology#DescriptiveInformationContentEntity">
        <rdfs:subClassOf rdf:resource="http://www.ontologylibrary.mil/CommonCore/Mid/InformationEntityOntology#InformationContentEntity"/>
        <obo:IAO_0000115>An Information Content Entity that consists of a set of propositions that describe some Entity.</obo:IAO_0000115>
        <rdfs:label>Descriptive Information Content Entity</rdfs:label>
    </owl:Class>
    


    <!-- http://www.ontologylibrary.mil/CommonCore/Mid/InformationEntityOntology#InformationContentEntity -->

    <owl:Class rdf:about="http://www.ontologylibrary.mil/CommonCore/Mid/InformationEntityOntology#InformationContentEntity">
        <rdfs:subClassOf rdf:resource="http://purl.obolibrary.org/obo/BFO_0000031"/>
        <obo:IAO_0000115>A Generically Dependent Continuant that generically depends on some Information Bearing Entity and stands in relation of aboutness to some Entity.</obo:IAO_0000115>
        <rdfs:label>Information Content Entity</rdfs:label>
    </owl:Class>
    


    <!-- http://www.semanticweb.org/lenovo/ontologies/2017/10/memon_00001003 -->

    <owl:Class rdf:about="http://www.semanticweb.org/lenovo/ontologies/2017/10/memon_00001003">
        <rdfs:subClassOf rdf:resource="http://www.ontologylibrary.mil/CommonCore/Mid/ArtifactOntology#Transducer"/>
        <rdfs:subClassOf>
            <owl:Restriction>
                <owl:onProperty rdf:resource="http://www.semanticweb.org/lenovo/ontologies/2017/10/memon_00001060"/>
                <owl:someValuesFrom rdf:resource="http://www.semanticweb.org/lenovo/ontologies/2017/10/memon_00001058"/>
            </owl:Restriction>
        </rdfs:subClassOf>
        <obo:IAO_0000115>A Transducer that is designed to detect events or changes in its environment, and then provide a corresponding output. It can be a sensor, a satellite, or a sensor system.</obo:IAO_0000115>
        <rdfs:label xml:lang="fr">sensing system</rdfs:label>
    </owl:Class>
    


    <!-- http://www.semanticweb.org/lenovo/ontologies/2017/10/memon_00001057 -->

    <owl:Class rdf:about="http://www.semanticweb.org/lenovo/ontologies/2017/10/memon_00001057">
        <rdfs:subClassOf rdf:resource="http://www.semanticweb.org/lenovo/ontologies/2017/10/memon_00001003"/>
        <obo:IAO_0000115>A satellite is an object which has been sent into space in order to collect information or to be part of a communications system. Satellites move continually round the Earth or around another planet.</obo:IAO_0000115>
        <rdfs:label xml:lang="fr">satellite</rdfs:label>
    </owl:Class>
    


    <!-- http://www.semanticweb.org/lenovo/ontologies/2017/10/memon_00001058 -->

    <owl:Class rdf:about="http://www.semanticweb.org/lenovo/ontologies/2017/10/memon_00001058">
        <rdfs:subClassOf rdf:resource="http://www.ontologylibrary.mil/CommonCore/Mid/ArtifactOntology#Transducer"/>
        <obo:IAO_0000115 xml:lang="en">An Entity to which other Entities can be attached - particuarly Sensors and other Platforms.  For example, a post might act as the Platform, a bouy might act as a Platform, or a fish might act as a Platform for an attached sensor.</obo:IAO_0000115>
        <rdfs:label xml:lang="fr">platform</rdfs:label>
    </owl:Class>
    


    <!-- http://www.semanticweb.org/lenovo/ontologies/2017/10/memon_00001061 -->

    <owl:Class rdf:about="http://www.semanticweb.org/lenovo/ontologies/2017/10/memon_00001061">
        <rdfs:subClassOf rdf:resource="http://www.ontologylibrary.mil/CommonCore/Mid/InformationEntityOntology#DescriptiveInformationContentEntity"/>
        <rdfs:subClassOf>
            <owl:Restriction>
                <owl:onProperty rdf:resource="http://www.semanticweb.org/lenovo/ontologies/2017/10/memon_00001064"/>
                <owl:allValuesFrom rdf:resource="http://www.semanticweb.org/lenovo/ontologies/2017/10/memon_00001003"/>
            </owl:Restriction>
        </rdfs:subClassOf>
        <rdfs:label xml:lang="fr">sensing system output</rdfs:label>
    </owl:Class>
    


    <!-- http://www.semanticweb.org/lenovo/ontologies/2017/10/memon_00001062 -->

    <owl:Class rdf:about="http://www.semanticweb.org/lenovo/ontologies/2017/10/memon_00001062">
        <rdfs:subClassOf rdf:resource="http://www.semanticweb.org/lenovo/ontologies/2017/10/memon_00001061"/>
        <rdfs:subClassOf>
            <owl:Restriction>
                <owl:onProperty rdf:resource="http://www.semanticweb.org/lenovo/ontologies/2017/10/memon_00001064"/>
                <owl:allValuesFrom rdf:resource="http://www.ontologylibrary.mil/CommonCore/Mid/ArtifactOntology#Sensor"/>
            </owl:Restriction>
        </rdfs:subClassOf>
        <rdfs:label xml:lang="fr">sensor output</rdfs:label>
    </owl:Class>
    


    <!-- http://www.semanticweb.org/lenovo/ontologies/2017/10/memon_00001063 -->

    <owl:Class rdf:about="http://www.semanticweb.org/lenovo/ontologies/2017/10/memon_00001063">
        <rdfs:subClassOf rdf:resource="http://www.semanticweb.org/lenovo/ontologies/2017/10/memon_00001061"/>
        <rdfs:subClassOf>
            <owl:Restriction>
                <owl:onProperty rdf:resource="http://www.semanticweb.org/lenovo/ontologies/2017/10/memon_00001064"/>
                <owl:allValuesFrom rdf:resource="http://www.semanticweb.org/lenovo/ontologies/2017/10/memon_00001057"/>
            </owl:Restriction>
        </rdfs:subClassOf>
        <rdfs:label xml:lang="fr">satellite output</rdfs:label>
    </owl:Class>
    


    <!-- http://www.semanticweb.org/lenovo/ontologies/2017/10/memon_00001065 -->

    <owl:Class rdf:about="http://www.semanticweb.org/lenovo/ontologies/2017/10/memon_00001065">
        <rdfs:subClassOf rdf:resource="http://www.ontologylibrary.mil/CommonCore/Mid/ArtifactOntology#Sensor"/>
        <obo:IAO_0000115>A rain sensor or rain switch is a switching device activated by rainfall.</obo:IAO_0000115>
        <rdfs:label xml:lang="fr">rain sensor</rdfs:label>
    </owl:Class>
    


    <!-- http://www.semanticweb.org/lenovo/ontologies/2017/10/memon_00001066 -->

    <owl:Class rdf:about="http://www.semanticweb.org/lenovo/ontologies/2017/10/memon_00001066">
        <rdfs:subClassOf rdf:resource="http://www.ontologylibrary.mil/CommonCore/Mid/ArtifactOntology#Sensor"/>
        <obo:IAO_0000115>A seismometer is an instrument that measures motion of the ground, caused by, for example, an earthquake, a volcanic eruption, or the use of explosives.</obo:IAO_0000115>
        <rdfs:label xml:lang="fr">seismometer</rdfs:label>
    </owl:Class>
    


    <!-- http://www.semanticweb.org/lenovo/ontologies/2017/10/memon_00001067 -->

    <owl:Class rdf:about="http://www.semanticweb.org/lenovo/ontologies/2017/10/memon_00001067">
        <rdfs:subClassOf rdf:resource="http://www.ontologylibrary.mil/CommonCore/Mid/ArtifactOntology#Sensor"/>
        <obo:IAO_0000115>A snow gauge is a type of instrument used by meteorologists and hydrologists  to gather and measure the amount of solid precipitation (as opposed to liquid precipitation that is measured by a rain gauge) over a set period of time</obo:IAO_0000115>
        <rdfs:label xml:lang="fr">snow gauge</rdfs:label>
    </owl:Class>
    


    <!-- http://www.semanticweb.org/lenovo/ontologies/2017/10/memon_00001068 -->

    <owl:Class rdf:about="http://www.semanticweb.org/lenovo/ontologies/2017/10/memon_00001068">
        <rdfs:subClassOf rdf:resource="http://www.ontologylibrary.mil/CommonCore/Mid/ArtifactOntology#Sensor"/>
        <obo:IAO_0000115>Soil moisture sensors measure the volumetric water content in soil.</obo:IAO_0000115>
        <rdfs:label xml:lang="fr">soil moisture sensor</rdfs:label>
    </owl:Class>
    


    <!-- http://www.semanticweb.org/lenovo/ontologies/2017/10/memon_00001069 -->

    <owl:Class rdf:about="http://www.semanticweb.org/lenovo/ontologies/2017/10/memon_00001069">
        <rdfs:subClassOf rdf:resource="http://www.ontologylibrary.mil/CommonCore/Mid/ArtifactOntology#Sensor"/>
        <obo:IAO_0000115>An air flow meter, is a device that measures air flow, i.e. how much air is flowing through a tube.</obo:IAO_0000115>
        <rdfs:label xml:lang="fr">air flow meter</rdfs:label>
    </owl:Class>
    


    <!-- http://www.semanticweb.org/lenovo/ontologies/2017/10/memon_00001070 -->

    <owl:Class rdf:about="http://www.semanticweb.org/lenovo/ontologies/2017/10/memon_00001070">
        <rdfs:subClassOf rdf:resource="http://www.ontologylibrary.mil/CommonCore/Mid/ArtifactOntology#Sensor"/>
        <obo:IAO_0000115>Water meters are used to measure the volume of water used by residential and commercial buildings that are supplied with water by a public water supply system. Water meters can also be used at the water source, well, or throughout a water system to determine flow through a particular portion of the system.</obo:IAO_0000115>
        <rdfs:label xml:lang="fr">water meter</rdfs:label>
    </owl:Class>
    


    <!-- http://www.semanticweb.org/lenovo/ontologies/2017/10/memon_00001071 -->

    <owl:Class rdf:about="http://www.semanticweb.org/lenovo/ontologies/2017/10/memon_00001071">
        <rdfs:subClassOf rdf:resource="http://www.ontologylibrary.mil/CommonCore/Mid/ArtifactOntology#Sensor"/>
        <obo:IAO_0000115>A pressure sensor is a device for pressure measurement of gases or liquids</obo:IAO_0000115>
        <rdfs:label xml:lang="fr">pressure sensor</rdfs:label>
    </owl:Class>
    


    <!-- http://www.semanticweb.org/lenovo/ontologies/2017/10/memon_00001072 -->

    <owl:Class rdf:about="http://www.semanticweb.org/lenovo/ontologies/2017/10/memon_00001072">
        <rdfs:subClassOf rdf:resource="http://www.ontologylibrary.mil/CommonCore/Mid/ArtifactOntology#Sensor"/>
        <obo:IAO_0000115>A temperature sensor or a thermometer is a device that measures temperature or a temperature gradient. Thermometers are widely used in industry to monitor processes, in meteorology, in medicine, and in scientific research.</obo:IAO_0000115>
        <rdfs:label xml:lang="fr">temperature sensor</rdfs:label>
    </owl:Class>
    


    <!-- http://www.semanticweb.org/lenovo/ontologies/2017/10/memon_00001104 -->

    <owl:Class rdf:about="http://www.semanticweb.org/lenovo/ontologies/2017/10/memon_00001104">
        <rdfs:subClassOf rdf:resource="http://www.ontologylibrary.mil/CommonCore/Mid/ArtifactOntology#Sensor"/>
        <obo:IAO_0000115>A rain gauge (also known as an udometer, pluviometer, or an ombrometer) is an instrument used by meteorologists and hydrologists to gather and measure the amount of liquid precipitation over a set period of time.</obo:IAO_0000115>
        <rdfs:label xml:lang="fr">rain gauge</rdfs:label>
    </owl:Class>
</rdf:RDF>



<!-- Generated by the OWL API (version 4.2.5.20160517-0735) https://github.com/owlcs/owlapi -->

